Proved new_chan spec (but add a stronger side-condition)

theories/channel/multi_channel.v
@@ -28,22 +28,19 @@ From actris.channel Require Import multi_proto_model.
 From actris.channel Require Export multi_proto.
 Set Default Proof Using "Type".
 
-(* TODO: Update new_chan definition to use pointers with offsets *)
 (** * The definition of the message-passing connectives *)
 Definition new_chan : val :=
-  λ: "n",
-    let: "l" := AllocN ("n"*"n") NONEV in
-    let: "xxs" := AllocN "n" NONEV in
-    (rec: "go1" "i" := if: "i" = "n" then #() else
-       let: "xs" := AllocN "n" NONEV in
-       (rec: "go2" "j" := if: "j" = "n" then #() else
-          ("xs" +ₗ "j") <- ("l" +ₗ ("i"*"n"+"j"), "l" +ₗ ("j"*"n"+"i"));;
-          "go2" ("j"+#1)) #0;;
-       ("xxs" +ₗ "i") <- "xs";;
-       "go1" ("i"+#1)) #0;; "xxs".
+  λ: "n", (AllocN ("n"*"n") NONEV, "n").
 
 Definition get_chan : val :=
-  λ: "cs" "i", ! ("cs" +ₗ "i").
+  λ: "cs" "i", ("cs","i").
+
+Definition diverge : val :=
+  λ: <>, (rec: "go" <> := "go" #())%V #().
+
+Definition guard : val :=
+  λ: "i" "n",
+    if: "i" < "n" then #() else diverge #().
 
 Definition wait : val :=
   rec: "go" "c" :=
@@ -52,27 +49,30 @@ Definition wait : val :=
     | SOME <> => "go" "c"
     end.
 
-Definition send : val :=
-  λ: "c" "i" "v",
-    let: "len" := Fst "c" in
-    if: "i" < "len" then
-      let: "l" := Fst (! ((Snd "c") +ₗ "i")) in
-      "l" <- SOME "v";; wait "l"
-    (* OBS: Hacky *)
-    else (rec: "go" <> := "go" #())%V #().
 
+Definition pos (n i j : nat) : nat := i * n + j.
+Definition vpos : val := λ: "n" "i" "j", "i"*"n" + "j".
+
+Definition send : val :=
+  λ: "c" "j" "v",
+    let: "n" := Snd (Fst "c") in guard "j" "n";;
+    let: "ls" := Fst (Fst "c") in
+    let: "i" := Snd "c" in
+    let: "l" := "ls" +ₗ vpos "n" "i" "j" in
+    "l" <- SOME "v";; wait "l".
+
+(* TODO: Move recursion further in *)
 Definition recv : val :=
-  rec: "go" "c" "i" :=
-    let: "len" := Fst "c" in
-    if: "i" < "len" then
-      let: "l" := Snd (! ((Snd "c") +ₗ "i")) in
-      let: "v" := Xchg "l" NONEV in
-      match: "v" with
-        NONE => "go" "c" "i"
-      | SOME "v" => "v"
-      end
-    (* OBS: Hacky *)
-    else (rec: "go" <> := "go" #())%V #().
+  rec: "go" "c" "j" :=
+    let: "n" := Snd (Fst "c") in guard "j" "n";;
+    let: "ls" := Fst (Fst "c") in
+    let: "i" := Snd "c" in
+    let: "l" := "ls" +ₗ vpos "n" "j" "i" in
+    let: "v" := Xchg "l" NONEV in
+    match: "v" with
+      NONE     => "go" "c" "j"
+    | SOME "v" => "v"
+    end.
 
 (** * Setup of Iris's cameras *)
 Class proto_exclG Σ V :=
@@ -99,7 +99,7 @@ Notation iMsg Σ := (iMsg Σ val).
 Definition tok `{!chanG Σ} (γ : gname) : iProp Σ := own γ (Excl ()).
 
 Definition chan_inv `{!heapGS Σ, !chanG Σ} γ γE γt i j (l:loc) : iProp Σ :=
-  (l ↦ NONEV ∗ tok γt) ∨
+  (l ↦ NONEV ∗ tok γt)%I ∨
   (∃ v m, l ↦ SOMEV v ∗
             iProto_own γ i (<(Send, j)> m)%proto ∗
             (∃ p, iMsg_car m v (Next p) ∗ own γE (●E (Next p)))) ∨
@@ -108,15 +108,13 @@ Definition chan_inv `{!heapGS Σ, !chanG Σ} γ γE γt i j (l:loc) : iProp Σ :
 
 Definition iProto_pointsto_def `{!heapGS Σ, !chanG Σ}
     (c : val) (p : iProto Σ) : iProp Σ :=
-  ∃ γ γE1 γE2 γt1 γt2 i (l:loc) ls p',
-    ⌜ c = PairV #(length ls) #l ⌝ ∗
+  ∃ γ γE1 (l:loc) (i:nat) (n:nat) p',
+    ⌜ c = (#l,#n,#i)%V ⌝ ∗
     inv (nroot.@"ctx") (iProto_ctx γ) ∗
-    l ↦∗ ls ∗
-    ([∗list] j ↦ v ∈ ls, 
-       ∃ (l1 l2 : loc),
-         ⌜v = PairV #l1 #l2⌝ ∗
-         inv (nroot.@"p") (chan_inv γ γE1 γt1 i j l1) ∗
-         inv (nroot.@"p") (chan_inv γ γE2 γt2 j i l2)) ∗
+    ([∗list] j ↦ _ ∈ replicate n (), 
+       ∃ γE2 γt1 γt2,
+         inv (nroot.@"p") (chan_inv γ γE1 γt1 i j (l +ₗ (pos n i j))) ∗
+         inv (nroot.@"p") (chan_inv γ γE2 γt2 j i (l +ₗ (pos n j i)))) ∗
     ▷ (p' ⊑ p) ∗
     own γE1 (●E (Next p')) ∗ own γE1 (◯E (Next p')) ∗
     iProto_own γ i p'.
@@ -131,10 +129,18 @@ Notation "c ↣ p" := (iProto_pointsto c p)
 
 Definition chan_pool `{!heapGS Σ, !chanG Σ}
     (cs : val) (ps : gmap nat (iProto Σ)) : iProp Σ :=
-  ∃ (l:loc) (ls : list val),
-    ⌜cs = #l⌝ ∗ ⌜∀ i, is_Some (ps !! i) → is_Some (ls !! i)⌝ ∗
-    l ↦∗ ls ∗
-    [∗list] i ↦ c ∈ ls, (∀ p, ⌜ps !! i = Some p⌝ -∗ c ↣ p).
+  ∃ γ (γEs : list gname) (l:loc) (n:nat),
+    ⌜cs = (#l,#n)%V⌝ ∗ ⌜∀ i, is_Some (ps !! i) → i < n⌝ ∗
+    inv (nroot.@"ctx") (iProto_ctx γ) ∗
+    [∗ list] i ↦ _ ∈ replicate n (),
+      (∀ p, ⌜ps !! i = Some p⌝ -∗
+            own (γEs !!! i) (●E (Next p)) ∗
+            own (γEs !!! i) (◯E (Next p)) ∗
+            iProto_own γ i p) ∗    
+      [∗ list] j ↦ _ ∈ replicate n (),
+        ∃ γt1 γt2,
+        inv (nroot.@"p") (chan_inv γ (γEs !!! i) γt1 i j (l +ₗ (pos n i j))) ∗
+        inv (nroot.@"p") (chan_inv γ (γEs !!! j) γt2 j i (l +ₗ (pos n j i))).
 
 Section channel.
   Context `{!heapGS Σ, !chanG Σ}.
@@ -150,20 +156,185 @@ Section channel.
   Proof.
     rewrite iProto_pointsto_eq.
     iDestruct 1 as
-      (γ γE1 γE2 γt1 γt2 i l ls p ->) "(#IH & Hl & Hls & Hle & H● & H◯ & Hown)".
-    iIntros "Hle'". iExists γ, γE1, γE2, γt1, γt2, i, l, ls, p.
+      (γ γE l n i p ->) "(#IH & Hls & Hle & H● & H◯ & Hown)".
+    iIntros "Hle'". iExists γ, γE, l, n, i, p.
     iSplit; [done|]. iFrame "#∗".
     iApply (iProto_le_trans with "Hle Hle'").
   Qed.
 
+  Lemma big_sepL_replicate {A B} n (x1 : A) (x2 : B) (P : nat → iProp Σ) :
+    ([∗ list] i ↦ _ ∈ replicate n x1, P i) ⊢
+    ([∗ list] i ↦ _ ∈ replicate n x2, P i).
+  Proof.
+    iIntros "H".
+    iInduction n as [|n] "IHn".
+    { done. }
+    replace (S n) with (n + 1) by lia.
+    rewrite !replicate_add. 
+    simpl. iDestruct "H" as "[H1 H2]".
+    iSplitL "H1".
+    { by iApply "IHn". }
+    simpl. rewrite !replicate_length. iFrame.
+  Qed.
+    
+  Lemma array_to_matrix_pre l n m v :
+    l ↦∗ replicate (n * m) v -∗
+    [∗ list] i ↦ _ ∈ replicate n (),
+      (l +ₗ i*m) ↦∗ replicate m v.
+  Proof.
+    iIntros "Hl".
+    iInduction n as [|n] "IHn".
+    { done. }
+    replace (S n) with (n + 1) by lia.
+    replace ((n + 1) * m) with (n * m + m) by lia.
+    rewrite !replicate_add. simpl.
+    rewrite array_app.
+    iDestruct "Hl" as "[H1 H2]".
+    iDestruct ("IHn" with "H1") as "H1".
+    iFrame.
+    simpl. 
+    rewrite Nat.add_0_r.
+    rewrite !replicate_length.
+    replace (Z.of_nat (n * m)) with (Z.of_nat n * Z.of_nat m)%Z by lia.
+    iFrame.
+  Qed.
+
+  Lemma array_to_matrix l n v :
+    l ↦∗ replicate (n * n) v -∗
+    [∗ list] i ↦ _ ∈ replicate n (),
+      [∗ list] j ↦ _ ∈ replicate n (),
+        (l +ₗ pos n i j) ↦ v.
+  Proof.
+    iIntros "H".
+    iDestruct (array_to_matrix_pre with "H") as "H".
+    iApply (big_sepL_impl with "H").
+    iIntros "!>" (i ? HSome) "H".
+    clear HSome.
+    rewrite /array.
+    iApply big_sepL_replicate.
+    iApply (big_sepL_impl with "H").
+    iIntros "!>" (j ? HSome) "Hl".
+    rewrite /pos.
+    rewrite Loc.add_assoc. 
+    replace (Z.of_nat i * Z.of_nat n + Z.of_nat j)%Z with
+      (Z.of_nat (i * n + j))%Z by lia.
+    apply lookup_replicate in HSome as [-> _]. done.
+  Qed.
+
   (** ** Specifications of [send] and [recv] *)
   Lemma new_chan_spec (n:nat) (ps:gmap nat (iProto Σ)) :
-    (∀ i, i < n → is_Some (ps !! i)) →
-    n = (size (dom ps)) →
+    0 < n →
+    (∀ i, i < n ↔ is_Some (ps !! i)) →     (* TODO: Weaken this! *)
+    (* n = (size (dom ps)) → *)
     {{{ iProto_consistent ps }}}
       new_chan #n
     {{{ cs, RET cs; chan_pool cs ps }}}.
-  Proof. Admitted.
+  Proof.
+    iIntros (Hle HSome Φ) "Hps HΦ". wp_lam.
+    wp_smart_apply wp_allocN; [lia|done|].
+    iIntros (l) "[Hl _]".
+    iMod (iProto_init with "Hps") as (γ) "[Hps Hps']".
+    wp_pures. iApply "HΦ".
+    iAssert (|==> ∃ (γEs : list gname),
+                ⌜length γEs = n⌝ ∗ 
+                [∗ list] i ↦ _ ∈ replicate n (),
+                  own (γEs !!! i) (●E (Next (ps !!! i))) ∗
+                  own (γEs !!! i) (◯E (Next (ps !!! i))) ∗
+                  iProto_own γ i (ps !!! i))%I with "[Hps']" as "H".
+    { clear Hle.
+      (* iInduction n as [|n] "IHn" forall (ps HSome Heq). *)
+      iInduction n as [|n] "IHn" forall (ps HSome).
+      { iExists []. iModIntro. simpl. done. }
+      assert (n < S n) by lia.
+      apply HSome in H. destruct H as [p ?]. 
+      iDestruct (big_sepM_delete _ _ n with "Hps'") as "[Hp Hps']".
+      { done. }
+      iMod (own_alloc (●E (Next p) ⋅ ◯E (Next p))) as (γE) "[Hauth Hfrag]".
+      { apply excl_auth_valid. }
+      iMod ("IHn" with "[] Hps'") as (γEs Hlen) "H".
+      { iPureIntro.
+        intros i.
+        split.
+        - intros Hle. 
+          rewrite lookup_delete_ne; [|lia].
+          apply HSome. lia.
+        - intros HSome'. 
+          destruct (decide (i=n)).
+          + simplify_eq. rewrite lookup_delete in HSome'. by inversion HSome'.
+          + rewrite lookup_delete_ne in HSome'; [|lia]. apply HSome in HSome'.
+            lia.
+      }        
+      iModIntro. iExists (γEs++[γE]).
+      replace (S n) with (n + 1) by lia.
+      rewrite replicate_add.
+      rewrite big_sepL_app.
+      rewrite app_length.
+      rewrite Hlen. iSplit; [done|].
+      simpl.
+      iSplitL "H".
+      { iApply (big_sepL_impl with "H").
+        iIntros "!>" (i ? HSome') "(Hauth & Hfrag & Hown)".
+        assert (i < n).
+        { by apply lookup_replicate_1 in HSome' as [? ?]. }
+        assert (delete n ps !!! i = ps !!! i) as Heq'.
+        { apply lookup_total_delete_ne. lia. }          
+        rewrite Heq'. iFrame.
+        rewrite lookup_total_app_l; [|lia]. iFrame. }
+      simpl. rewrite replicate_length. rewrite Nat.add_0_r.
+      rewrite list_lookup_total_middle; [|done].
+      rewrite lookup_total_alt. rewrite H. simpl. iFrame. }
+    iMod "H" as (γEs Hlen) "H".
+    iAssert (|={⊤}=>
+        [∗ list] i ↦ _ ∈ replicate n (),
+          [∗ list] j ↦ _ ∈ replicate n (),
+            ∃ γt,
+            inv (nroot.@"p") (chan_inv γ (γEs !!! i) γt i j
+                                       (l +ₗ (pos n i j))))%I with "[Hl]" as "IH".
+    { replace (Z.to_nat (Z.of_nat n * Z.of_nat n)) with (n*n) by lia.
+      iDestruct (array_to_matrix with "Hl") as "Hl".
+      iApply big_sepL_fupd.
+      iApply (big_sepL_impl with "Hl").
+      iIntros "!>" (i ? HSome') "H1".
+      iApply big_sepL_fupd.
+      iApply (big_sepL_impl with "H1").
+      iIntros "!>" (j ? HSome'') "H1".
+      iMod (own_alloc (Excl ())) as (γ') "Hγ'".
+      { done. }
+      iExists γ'.
+      iApply inv_alloc.
+      iLeft. iFrame. }
+    iMod "IH" as "#IH".
+    iMod (inv_alloc with "Hps") as "#IHp".
+    iExists _,_,_,_.
+    iModIntro. iSplit; [done|].
+    iSplit.
+    { iPureIntro. intros. apply HSome in H. done. } 
+    iFrame "IHp".
+    iApply (big_sepL_impl with "H").
+    iIntros "!>" (i ? HSome') "(Hauth & Hfrag & Hown)".
+    iSplitL.
+    { iIntros (p HSome'').
+      rewrite lookup_total_alt. rewrite HSome''.
+      iFrame. }
+    iApply big_sepL_intro.
+    iIntros "!>" (j ? HSome'').
+    assert (i < n) as Hle'.
+    { apply lookup_replicate in HSome' as [_ Hle']. done. }
+    assert (j < n) as Hle''.
+    { apply lookup_replicate in HSome'' as [_ Hle'']. done. }
+    iDestruct (big_sepL_lookup _ _ i () with "IH") as "IH''".
+    { rewrite lookup_replicate. done. }
+    iDestruct (big_sepL_lookup _ _ j () with "IH''") as "IH'''".
+    { rewrite lookup_replicate. done. }
+    iFrame "#".
+    iDestruct (big_sepL_lookup _ _ j () with "IH") as "H".
+    { rewrite lookup_replicate. done. }
+    iDestruct (big_sepL_lookup _ _ i () with "H") as "H'".
+    { rewrite lookup_replicate. done. }
+    iDestruct "IH'''" as (γ1) "?".
+    iDestruct "H'" as (γ2) "?".
+    iExists _, _. iFrame "#".
+  Qed.
 
   Lemma get_chan_spec cs (i:nat) ps p :
     ps !! i = Some p →
@@ -172,30 +343,37 @@ Section channel.
     {{{ c, RET c; c ↣ p ∗ chan_pool cs (delete i ps) }}}.
   Proof.
     iIntros (HSome Φ) "Hcs HΦ".
-    iDestruct "Hcs" as (l ls -> Hlen) "[Hl Hls]".
-    wp_lam.
-    assert (is_Some (ls !! i)) as [c HSome'].
-    { by apply Hlen. }
-    wp_smart_apply (wp_load_offset with "Hl"); [done|].
-    iIntros "Hcs".
+    iDestruct "Hcs" as (γp γEs l n -> Hle) "[#IHp Hl]".
+    wp_lam. wp_pures.
+    assert (i < n).
+    { apply Hle. eexists _. done. }
+    iDestruct (big_sepL_delete _ _ i () with "Hl") as "[[Hi #IHs] H]".
+    { by apply lookup_replicate. }
+    iDestruct ("Hi" with "[//]") as "(Hauth & Hown & Hp)". 
+    iModIntro.
     iApply "HΦ".
-    iDestruct (big_sepL_delete' _ _ i with "Hls") as "[Hc Hls]"; [set_solver|].
-    iDestruct ("Hc" with "[//]") as "Hc".
-    iFrame.
-    iExists _, _. iSplit; [done|]. iFrame "Hcs".
-    iSplitR.
-    { iPureIntro. intros j HSome''.
-      destruct (decide (i=j)) as [<-|Hneq].
-      { rewrite lookup_delete in HSome''. done. }
-      rewrite lookup_delete_ne in HSome''; [|done].
-      by apply Hlen. }
-    iApply (big_sepL_impl with "Hls").
-    iIntros "!>" (j v Hin) "H".
-    iIntros (p' HSome'').
-    destruct (decide (i=j)) as [<-|Hneq].
-    { rewrite lookup_delete in HSome''. done. }
-    rewrite lookup_delete_ne in HSome''; [|done].
-    by iApply "H".
+    iSplitR "H".
+    { rewrite iProto_pointsto_eq.
+      iExists _, _, _, _, _, _.
+      iSplit; [done|].
+      iFrame "#∗". iSplit; [|iNext; done].
+      iApply (big_sepL_impl with "IHs").
+      iIntros "!>" (???). iDestruct 1 as (γt1 γt2) "[H1 H2]".
+      iExists _,_,_. iFrame. }
+    iExists _, _, _, _.
+    iSplit; [done|].
+    iSplit.
+    { iPureIntro. intros i' HSome'. apply Hle.
+      assert (i ≠ i').
+      { intros ->. rewrite lookup_delete in HSome'. by inversion HSome'. } 
+      rewrite lookup_delete_ne in HSome'; done. }
+    iFrame "#∗".
+    iApply (big_sepL_impl with "H").
+    iIntros "!>" (i' ? HSome'').
+    case_decide.
+    { simplify_eq. iFrame "#".
+      iIntros "_" (p' Hin). simplify_eq. by rewrite lookup_delete in Hin. }
+    rewrite lookup_delete_ne; [|done]. eauto.
   Qed.
 
   Lemma own_prot_excl γ i (p1 p2 : iProto Σ) :
@@ -206,6 +384,33 @@ Section channel.
     iIntros "Hi Hj". by iDestruct (own_prot_idx with "Hi Hj") as %Hneq.
   Qed.
 
+  Lemma diverge_spec P : 
+    {{{ True }}} diverge #() {{{ RET #(); P }}}.
+  Proof.
+    iIntros (Φ) "_ HΦ". 
+    wp_lam. iLöb as "IH".
+    wp_pures. by iApply "IH".
+  Qed.
+
+  Lemma guard_spec (i n : nat) : 
+    {{{ True }}} guard #i #n {{{ RET #(); ⌜i < n⌝ }}}.
+  Proof.
+    iIntros (Φ) "_ HΦ". 
+    wp_lam. wp_pures. 
+    case_bool_decide.
+    - wp_pures. iApply "HΦ". iPureIntro. lia. 
+    - by wp_smart_apply diverge_spec. 
+  Qed.
+
+  Lemma vpos_spec (n i j : nat) : 
+    {{{ True }}} vpos #n #i #j {{{ RET #(pos n i j); True }}}.
+  Proof.
+    iIntros (Φ) "_ HΦ". wp_lam. wp_pures. rewrite /pos.
+    replace (Z.of_nat i * Z.of_nat n + Z.of_nat j)%Z with
+      (Z.of_nat (i * n + j)) by lia.
+    by iApply "HΦ".
+  Qed.
+
   Lemma send_spec c j v p :
     {{{ c ↣ <(Send, j)> MSG v; p }}}
       send c #j v
@@ -213,27 +418,21 @@ Section channel.
   Proof.
     rewrite iProto_pointsto_eq. iIntros (Φ) "Hc HΦ". wp_lam; wp_pures.
     iDestruct "Hc" as
-      (γ γE1 γE2 γt1 γt2 i l ls p' ->) "(#IH & Hl & Hls & Hle & H● & H◯ & Hown)".
+      (γ γE l i n p' ->) "(#IH & #Hls & Hle & H● & H◯ & Hown)".
     wp_pures.
-    case_bool_decide; last first.
-    { wp_pures. iClear "IH H● H◯ Hown HΦ Hls Hl".
-      iLöb as "IH". wp_lam. iApply "IH". done. }
-    assert (is_Some (ls !! j)) as [l' HSome].
-    { apply lookup_lt_is_Some_2. lia. }
+    wp_smart_apply guard_spec; [done|].
+    iDestruct 1 as %Hle.
     wp_pures.
-    wp_smart_apply (wp_load_offset with "Hl").
-    { done. } 
-    iIntros "Hl". wp_pures.
-    iDestruct (big_sepL_lookup_acc with "Hls") as "[Hj Hls]"; [done|].
-    iDestruct "Hj" as (l1 l2 ->) "#[IHl1 IHl2]". 
-    iDestruct ("Hls" with "[]") as "Hls".
-    { iExists _, _. iFrame "#". done. }
+    wp_smart_apply (vpos_spec); [done|]. iIntros "_".
+    iDestruct (big_sepL_lookup_acc with "Hls") as "[Hj _]".
+    { by apply lookup_replicate_2. }
+    iDestruct "Hj" as (γE' γt γt') "#[IHl1 IHl2]". 
     wp_pures.
     wp_bind (Store _ _).
     iInv "IHl1" as "HIp".
     iDestruct "HIp" as "[HIp|HIp]"; last first.
     { iDestruct "HIp" as "[HIp|HIp]".
-      - iDestruct "HIp" as (? m) "(>Hl' & Hown' & HIp)".
+      - iDestruct "HIp" as (? m) "(>Hl & Hown' & HIp)".       
         wp_store.
         rewrite /iProto_own.
         iDestruct "Hown" as (p'') "[Hle' Hown]".
@@ -268,7 +467,7 @@ Section channel.
       wp_load. iModIntro.
       iSplitL "Hl' Hown HIp".
       { iRight. iLeft. iExists _, _. iFrame. }
-      wp_pures. iApply ("HL" with "HΦ Hl Hls Htok H◯").
+      wp_pures. iApply ("HL" with "HΦ Htok H◯").
     - iDestruct "HIp" as (p'') "(>Hl' & Hown & H●)".
       wp_load.
       iModIntro.
@@ -281,11 +480,11 @@ Section channel.
       { apply excl_auth_update. }
       iModIntro.
       iApply "HΦ".
-      iExists _,_, _, _, _, _, _, _, _.
+      iExists _, _, _, _, _, _.
       iSplit; [done|]. iFrame "#∗".
       iRewrite -"Hagree'". iApply iProto_le_refl.
   Qed.
-  
+
   Lemma send_spec_tele {TT} c i (tt : TT)
         (v : TT → val) (P : TT → iProp Σ) (p : TT → iProto Σ) :
     {{{ c ↣ (<(Send,i) @.. x > MSG v x {{ P x }}; p x) ∗ P tt }}}
@@ -302,7 +501,6 @@ Section channel.
     by iApply (send_spec with "Hc").
   Qed.
 
-
   Lemma recv_spec {TT} c j (v : TT → val) (P : TT → iProp Σ) (p : TT → iProto Σ) :
     {{{ c ↣ <(Recv, j) @.. x> MSG v x {{ ▷ P x }}; p x }}}
       recv c #j
@@ -311,21 +509,16 @@ Section channel.
     iIntros (Φ) "Hc HΦ". iLöb as "HL". wp_lam.
     rewrite iProto_pointsto_eq.
     iDestruct "Hc" as
-      (γ γE1 γE2 γt1 γt2 i l ls p' ->) "(#IH & Hl & Hls & Hle & H● & H◯ & Hown)".
+      (γ γE l i n p' ->) "(#IH & #Hls & Hle & H● & H◯ & Hown)".
     wp_pures.
-    case_bool_decide; last first.
-    { wp_pures. iClear "IH H● H◯ Hown HΦ Hls Hl".
-      iLöb as "IH". wp_lam. iApply "IH". done. }
     wp_pures.
-    assert (is_Some (ls !! j)) as [l' HSome].
-    { apply lookup_lt_is_Some_2. lia. }
-    wp_smart_apply (wp_load_offset with "Hl").
-    { done. } 
-    iIntros "Hl". wp_pures.
-    iDestruct (big_sepL_lookup_acc with "Hls") as "[Hj Hls]"; [done|].
-    iDestruct "Hj" as (l1 l2 ->) "#[IHl1 IHl2]". 
-    iDestruct ("Hls" with "[]") as "Hls".
-    { iExists _, _. iFrame "#". done. }    
+    wp_smart_apply guard_spec; [done|].
+    iDestruct 1 as %Hle.
+    wp_pures.
+    wp_smart_apply (vpos_spec); [done|]. iIntros "_".
+    iDestruct (big_sepL_lookup_acc with "Hls") as "[Hj _]".
+    { by apply lookup_replicate_2. }
+    iDestruct "Hj" as (γE' γt γt') "#[IHl1 IHl2]". 
     wp_pures.
     wp_bind (Xchg _ _).
     iInv "IHl2" as "HIp".
@@ -335,16 +528,16 @@ Section channel.
       iModIntro.
       iSplitL "Hl' Htok".
       { iLeft. iFrame. }
-      wp_pures. iApply ("HL" with "[H● H◯ Hown Hls Hl Hle] HΦ").
-      iExists _, _, _, _, _, _, _, _, _. iSplit; [done|]. iFrame "#∗". }
+      wp_pures. iApply ("HL" with "[H● H◯ Hown Hle] HΦ").
+      iExists _, _, _, _, _, _. iSplit; [done|]. iFrame "#∗". }
     iDestruct "HIp" as "[HIp|HIp]"; last first.
     { iDestruct "HIp" as (p'') "[>Hl' [Hown' H◯']]".
       wp_xchg.
       iModIntro.
       iSplitL "Hl' Hown' H◯'".
       { iRight. iRight. iExists _. iFrame. }
-      wp_pures. iApply ("HL" with "[H● H◯ Hown Hls Hl Hle] HΦ").
-      iExists _, _, _, _, _, _, _, _, _. iSplit; [done|]. iFrame "#∗". }
+      wp_pures. iApply ("HL" with "[H● H◯ Hown Hle] HΦ").
+      iExists _, _, _, _, _, _. iSplit; [done|]. iFrame "#∗". }
     iDestruct "HIp" as (w m) "(>Hl' & Hown' & HIp)".
     iDestruct "HIp" as (p'') "[Hm Hp']".
     iInv "IH" as "Hctx".
@@ -365,7 +558,7 @@ Section channel.
     { apply excl_auth_update. }
     iModIntro. iApply "HΦ".
     iFrame.
-    iExists _, _, _, _, _, _, _, _, _. iSplit; [done|].
+    iExists _, _, _, _, _, _. iSplit; [done|].
     iRewrite "Hp". iFrame "#∗". iApply iProto_le_refl.
   Qed.
 
